Просуммируем по $n_{1}$ и $n_{2}$

\begin{equation*}
\begin{aligned}
	\sum_{n_1=0}^N \sum_{n_2=0}^{N-n_1}\diffp{H_{n_1,n_2}(u,t)}{t}=
	&-\lambda \sum_{n_1=0}^N\sum_{n_2=0}^{N-n_1}
	H_{n_1, n_2}(u,t)
	+j\sigma \sum_{n_1=0}^N\sum_{n_2=0}^{N-n_1}
	\overline{E}^N_{n_1+n_2}\diffp{H_{n_1, n_2}(u,t)}{u}-\\
	&-\mu_1 \sum_{n_1=0}^N\sum_{n_2=0}^{N-n_1}
	n_1 H_{n_1, n_2}(u,t)
	-\mu_2 \sum_{n_1=0}^N\sum_{n_2=0}^{N-n_1}
	n_2 H_{n_1, n_2}(u,t)+\\
	&+\mu_1 r_1 q \sum_{n_1=0}^N\sum_{n_2=0}^{N-n_1}
	n_1 H_{n_1, n_2}(u,t)
	+\mu_2 r_1 (1-q)\sum_{n_1=0}^N\sum_{n_2=0}^{N-n_1} 
	n_2 H_{n_1, n_2}(u,t)+\\
	&+\lambda e^{ju}\sum_{n_1=0}^N\sum_{n_2=0}^{N-n_1}
	E^N_{n_1+n_2}H_{n_1, n_2}(u,t)+\\
	&+\lambda q \sum_{n_1=0}^N\sum_{n_2=0}^{N-n_1}
	H_{n_1-1, n_2}(u,t)
	-j \sigma q e^{-ju}\sum_{n_1=0}^N\sum_{n_2=0}^{N-n_1}
	\diffp{H_{n_1-1, n_2}(u,t)}{u}+\\
	&+\lambda (1-q) \sum_{n_1=0}^N\sum_{n_2=0}^{N-n_1}
	H_{n_1, n_2-1}(u,t){u}
	-j \sigma (1-q) e^{-ju}\sum_{n_1=0}^N\sum_{n_2=0}^{N-n_1}
	\diffp{H_{n_1, n_2-1}(u,t)}{u}+\\
	&+\mu_1 r_0 \sum_{n_1=0}^N\sum_{n_2=0}^{N-n_1}
	(n_1+1) H_{n_1+1, n_2}(u,t)
	+\mu_1 r_2 e^{ju} \sum_{n_1=0}^N\sum_{n_2=0}^{N-n_1}
	(n_1+1) H_{n_1+1, n_2}(u,t)+\\
	&+\mu_2 r_0 \sum_{n_1=0}^N\sum_{n_2=0}^{N-n_1}
	(n_2+1) H_{n_1, n_2+1}(u,t)
	+\mu_2 r_2 e^{ju} \sum_{n_1=0}^N\sum_{n_2=0}^{N-n_1}
	(n_2+1) H_{n_1, n_2+1}(u,t)+\\
	&+\mu_1 r_1 (1-q) \sum_{n_1=0}^N\sum_{n_2=0}^{N-n_1}
	(n_1+1)H_{n_1+1, n_2-1}(u,t)+\\
	&+\mu_2 r_1 q \sum_{n_1=0}^N\sum_{n_2=0}^{N-n_1}
	(n_2+1)H_{n_1-1, n_2+1}(u,t).\\	
\end{aligned}
\end{equation*}

Преобразуем

\begin{equation*}
\begin{aligned}
	\sum_{n_1=0}^N\sum_{n_2=0}^{N-n_1} \diffp{H_{n_1,n_2}(u,t)}{t}=
	&-\lambda \sum_{n_1=0}^N\sum_{n_2=0}^{N-n_1} H_{n_1, n_2}(u,t)+
	 +j\sigma \sum_{n_1=0}^{N-1}\sum_{n_2=0}^{N-1-n_1} 
	 \diffp{H_{n_1, n_2}(u,t)}{u}-\\
	&-\mu_1 (r_0+r_2) \sum_{n_1=0}^N\sum_{n_2=0}^{N-n_1} n_1 H_{n_1, n_2}(u,t)
	 -\mu_2 (r_0+r_2)\sum_{n_1=0}^N\sum_{n_2=0}^{N-n_1} n_2 H_{n_1, n_2}(u,t)+\\
	&+\lambda e^{ju}\sum_{n_1=0}^N\sum_{n_2=N-n_1}^{N-n_1} 
	  H_{n_1, n_2}(u,t)+\\
	&+\lambda q \sum_{n_1=0}^{N-1}\sum_{n_2=0}^{N-1-n_2} 
	  H_{n_1, n_2}(u,t)
	 -j \sigma q e^{-ju} \sum_{n_1=0}^{N-1}\sum_{n_2=0}^{N-1-n_1} 
	   \diffp{H_{n_1, n_2}(u,t)}{u}+\\
	&+\lambda (1-q) \sum_{n_1=0}^{N-1}\sum_{n_2=0}^{N-1-n_1} 
	  H_{n_1, n_2}(u,t) 
	 -j \sigma (1-q) e^{-ju}\sum_{n_1=0}^{N-1}\sum_{n_2=0}^{N-1-n_1} 
	  \diffp{H_{n_1, n_2}(u,t)}{u}+\\
	&+\mu_1 r_0 \sum_{n_1=0}^N\sum_{n_2=0}^{N-n_1} 
	  n_1 H_{n_1, n_2}(u,t)
	+\mu_1 r_2 e^{ju}\sum_{n_1=0}^{N}\sum_{n_2=0}^{N-n_1} 
	  n_1 H_{n_1, n_2}(u,t)+\\
	&+\mu_2 r_0 \sum_{n_1=0}^N\sum_{n_2=0}^{N-n_1} 
	  n_2 H_{n_1, n_2}(u,t)
	 +\mu_2 r_2 e^{ju}\sum_{n_1=0}^{N}\sum_{n_2=0}^{N-n_1} 
	  n_2 H_{n_1, n_2}(u,t).\\
\end{aligned}
\end{equation*}

Приведем подобные слагаемые 

\begin{equation*}
\begin{aligned}
	\sum_{n_1=0}^N\sum_{n_2=0}^{N-n_1} \diffp{H_{n_1,n_2}(u,t)}{t}=
	&\lambda (e^{ju} - 1)\sum_{n_1=0}^N\sum_{n_2=N-n_1}^{N-n_1} 
	  H_{n_1, n_2}(u,t)-\\
	&-j \sigma q (e^{-ju}-1) \sum_{n_1=0}^{N-1}\sum_{n_2=0}^{N-1-n_1} 
	   \diffp{H_{n_1, n_2}(u,t)}{u}-\\
	&-j \sigma (1-q) (e^{-ju}-1)\sum_{n_1=0}^{N-1}\sum_{n_2=0}^{N-1-n_1} 
	  \diffp{H_{n_1, n_2}(u,t)}{u}+\\
	&+\mu_1 r_2 (e^{ju} -1)\sum_{n_1=0}^{N}\sum_{n_2=0}^{N-n_1} 
	n_1 H_{n_1, n_2}(u,t)
	+\mu_2 r_2 (e^{ju} -1)\sum_{n_1=0}^{N}\sum_{n_2=0}^{N-n_1} 
	n_2 H_{n_1, n_2}(u,t),\\
\end{aligned}
\end{equation*}

\begin{equation*}
	\begin{aligned}
		\sum_{n_1=0}^N\sum_{n_2=0}^{N-n_1} \diffp{H_{n_1,n_2}(u,t)}{t}=
		&\lambda (e^{ju} - 1)\sum_{n_1=0}^N\sum_{n_2=N-n_1}^{N-n_1} 
		H_{n_1, n_2}(u,t)-\\
		&- j \sigma(e^{-ju}-1)\sum_{n_1=0}^{N-1}\sum_{n_2=0}^{N-1-n_1} 
		\diffp{H_{n_1, n_2}(u,t)}{u}+\\
		&+\mu_1 r_2 (e^{ju} -1)\sum_{n_1=0}^{N}\sum_{n_2=0}^{N-n_1} 
		n_1 H_{n_1, n_2}(u,t)
		+\mu_2 r_2 (e^{ju} -1)\sum_{n_1=0}^{N}\sum_{n_2=0}^{N-n_1} 
		n_2 H_{n_1, n_2}(u,t).\\
	\end{aligned}
\end{equation*}

Вынесем $(e^{ju} - 1)$

\begin{equation*}
	\begin{aligned}
		\sum_{n_1=0}^N\sum_{n_2=0}^{N-n_1} \diffp{H_{n_1,n_2}(u,t)}{t}=
		&(e^{ju} - 1)\bigg\{\lambda \sum_{n_1=0}^N\sum_{n_2=N-n_1}^{N-n_1} 
		H_{n_1, n_2}(u,t)+\\
		&+ j \sigma e^{-ju}\sum_{n_1=0}^{N-1}\sum_{n_2=0}^{N-1-n_1} 
		\diffp{H_{n_1, n_2}(u,t)}{u}+\\
		&+\mu_1 r_2 \sum_{n_1=0}^{N}\sum_{n_2=0}^{N-n_1} 
		n_1 H_{n_1, n_2}(u,t)
		+\mu_2 r_2 \sum_{n_1=0}^{N}\sum_{n_2=0}^{N-n_1} 
		n_2 H_{n_1, n_2}(u,t)\bigg\}.\\
	\end{aligned}
\end{equation*}
