Сделаем следующие подстановки в \eqref{hFirstSystemOfEquations}
\begin{align*}
H_{n_{1}, n_{2}}(u,t)=e^{j\frac{u}{\sigma}x(\sigma t)}H_{n_{1}, n_{2}}^{(1)}(u,t)
\end{align*}
Получим систему
\begin{equation}
	\begin{split}\label{renameH1}
		\diffp{H_{n_{1}, n_{2}}^{(1)}c(u,t)}{t}+jux'(\sigma t)H_{n_{1}, n_{2}}^{(1)}(u,t)=
		&-(\lambda+\mu_{1}n_{1}+\mu_{2}n_{2})H_{n_{1}, n_{2}}^{(1)}(u,t) +\\
		&+ j\sigma \overline{E}_{n_{1}+n_{2}}^N\diffp{H_{n_{1}, n_{2}}^{(1)}(u,t)}{u}-x(\sigma t)\overline{E}_{n_{1}+n_{2}}^NH_{n_{1}, n_{2}}^{(1)}+\\
		&+\mu_{1}r_{1}q n_{1}H_{n_{1}, n_{2}}^{(1)}(u,t)+ \mu_{2}r_{1}(1-q)n_{2}H_{n_{1}, n_{2}}^{(1)}(u,t)+\\
		&+ \lambda e^{ju} E_{n_{1}+n_{2}}^N H_{n_{1}, n_{2}}^{(1)}(u,t)+\\
		&+\lambda qH_{n_{1}-1, n_{2}}^{(1)}(u,t) - j \sigma q  e^{-ju} \diffp{H_{n_{1}-1, n_{2}}^{(1)}(u,t)}{u}+\\
		&+ q  e^{-ju} x(\sigma t)H_{n_{1}-1, n_{2}}^{(1)}(u,t)+\\
		&+\lambda (1-q)H_{n_{1}, n_{2}-1}^{(1)}(u,t) - j \sigma (1-q) e^{-ju} \diff{H_{n_{1}, n_{2}-1}^{(1)}(u,t)}{u}+\\
		&+ (1-q) e^{-ju} x(\sigma t) H_{n_{1}, n_{2}-1}^{(1)}(u,t)\\
		&+ \mu_{1} r_{0}(n_{1}+1) H_{n_{1} +1 , n_{2}}^{(1)}(u,t)+\\
		& + \mu_{1} r_{2}  e^{ju}(n_{1}+1)H_{n_{1} + 1, n_{2}}^{(1)}(u,t)+\\
		&+ \mu_{2} r_{0}(n_{2}+1) H_{n_{1}, n_{2} + 1 }(u,t)+\\
		& + \mu_{2} r_{2}  e^{ju}(n_{2}+1) H_{n_{1}, n_{2} + 1}(u,t)+\\
		&+\mu_{1} r_{1}(1-q)(n_{1}+1) H_{n_{1} +1 , n_{2}-1}^{(1)}(u,t)+\\
		&+(n_{2}+1)\mu_{2} r_{1}q H_{n_{1} -1 , n_{2}+1}^{(1)}(u,t) ,\\
		\sum_{n_1=0}^N\sum_{n_2=0}^{N-n_1}\{ \diffp{H_{n_1,n_2}^{(1)}(u,t)}{t}+ju x'(\sigma t)H_{n_1,n_2}^{(1)}(u,t)\}=
		&(e^{ju} - 1)\bigg\{\lambda \sum_{n_1=0}^N\sum_{n_2=N-n_1}^{N-n_1} 
		H_{n_1, n_2}^{(1)}(u,t)+\\
		&+ e^{-ju}\sum_{n_1=0}^{N-1}\sum_{n_2=0}^{N-1-n_1} 
		\bigg[j\sigma \diffp{ H_{n_1, n_2}^{(1)}(u,t)}{u}-\\
		&-x(\sigma t)H_{n_1, n_2}^{(1)}(u,t)\bigg]+\\
		&+\mu_1 r_2 \sum_{n_1=0}^{N}\sum_{n_2=0}^{N-n_1} 
		n_1 H_{n_1, n_2}^{(1)}(u,t)+\\
		&+\mu_2 r_2 \sum_{n_1=0}^{N}\sum_{n_2=0}^{N-n_1} 
		n_2 H_{n_1, n_2}^{(1)}(u,t)\bigg\}\
	\end{split}
\end{equation}
С учетом \eqref{a(x)} перепишем систему \eqref{renameH1}
\begin{equation}\label{h1SystemOfEquation}
	\begin{split}
		\diffp{H_{n_{1}, n_{2}}^{(1)}c(u,t)}{t}+ju a(x) H_{n_{1}, n_{2}}^{(1)}(u,t)=
		&-(\lambda+\mu_{1}n_{1}+\mu_{2}n_{2})H_{n_{1}, n_{2}}^{(1)}(u,t) +\\
		&+ j\sigma \overline{E}_{n_{1}+n_{2}}^N\diffp{H_{n_{1}, n_{2}}^{(1)}(u,t)}{u}-x\overline{E}_{n_{1}+n_{2}}^NH_{n_{1}, n_{2}}^{(1)}+\\
		&+\mu_{1}r_{1}q n_{1}H_{n_{1}, n_{2}}^{(1)}(u,t)+ \mu_{2}r_{1}(1-q)n_{2}H_{n_{1}, n_{2}}^{(1)}(u,t)+\\
		&+ \lambda e^{ju} E_{n_{1}+n_{2}}^N H_{n_{1}, n_{2}}^{(1)}(u,t)+\\
		&+\lambda qH_{n_{1}-1, n_{2}}^{(1)}(u,t) - j \sigma q  e^{-ju} \diffp{H_{n_{1}-1, n_{2}}^{(1)}(u,t)}{u}+\\
		&+ q  e^{-ju} xH_{n_{1}-1, n_{2}}^{(1)}(u,t)+\\
		&+\lambda (1-q)H_{n_{1}, n_{2}-1}^{(1)}(u,t) - j \sigma (1-q) e^{-ju} \diff{H_{n_{1}, n_{2}-1}^{(1)}(u,t)}{u}+\\
		&+ (1-q) e^{-ju} x H_{n_{1}, n_{2}-1}^{(1)}(u,t)+\\
		&+ \mu_{1} r_{0}(n_{1}+1) H_{n_{1} +1 , n_{2}}^{(1)}(u,t)+\\
		& + \mu_{1} r_{2}  e^{ju}(n_{1}+1)H_{n_{1} + 1, n_{2}}^{(1)}(u,t)+\\
		&+ \mu_{2} r_{0}(n_{2}+1) H_{n_{1}, n_{2} + 1 }(u,t)+\\
		& + \mu_{2} r_{2}  e^{ju}(n_{2}+1) H_{n_{1}, n_{2} + 1}(u,t)+\\
		&+\mu_{1} r_{1}(1-q)(n_{1}+1) H_{n_{1} +1 , n_{2}-1}^{(1)}(u,t)+\\
		&+(n_{2}+1)\mu_{2} r_{1}q H_{n_{1} -1 , n_{2}+1}^{(1)}(u,t) ,\\
		\sum_{n_1=0}^N\sum_{n_2=0}^{N-n_1}\{ \diffp{H_{n_1,n_2}^{(1)}(u,t)}{t}+ju a(x) H_{n_1,n_2}^{(1)}(u,t)\}=
		&(e^{ju} - 1)\bigg\{\lambda \sum_{n_1=0}^N\sum_{n_2=N-n_1}^{N-n_1} 
		H_{n_1, n_2}^{(1)}(u,t)\\
		&+ e^{-ju}\sum_{n_1=0}^{N-1}\sum_{n_2=0}^{N-1-n_1} 
		\bigg[\sigma j\diffp{ H_{n_1, n_2}^{(1)}(u,t)}{u}-xH_{n_1, n_2}^{(1)}(u,t)\bigg]+\\
		&+\mu_1 r_2 \sum_{n_1=0}^{N}\sum_{n_2=0}^{N-n_1} 
		n_1 H_{n_1, n_2}^{(1)}(u,t)+\\
		&+\mu_2 r_2 \sum_{n_1=0}^{N}\sum_{n_2=0}^{N-n_1} 
		n_2 H_{n_1, n_2}^{(1)}(u,t)\bigg\}\
	\end{split}
\end{equation}