Найдем $x=x(\tau)$. Рассмотрим второе уравнение \eqref{fSystemOfEquations} в пределе $\varepsilon \rightarrow 0$.
\begin{align*}
\sum_{n_1=0}^N\sum_{n_2=0}^{N-n_1} \diffp{F_{n_{1}, n_{2}}(w,\tau)}{\tau}=
&jw\bigg\{\lambda \sum_{n_1=0}^N\sum_{n_2=N-n_1}^{N-n_1} 
F_{n_{1}, n_{2}}(w,\tau, \varepsilon)+\\s
&+ j\sum_{n_1=0}^{N-1}\sum_{n_2=0}^{N-1-n_1} 
\diffp{F_{n_{1}, n_{2}}(w,\tau)}{w}+\\
&+\mu_1 r_2 \sum_{n_1=0}^{N}\sum_{n_2=0}^{N-n_1} 
n_1 F_{n_{1}, n_{2}}(w,\tau)
+\mu_2 r_2 \sum_{n_1=0}^{N}\sum_{n_2=0}^{N-n_1} 
n_2 F_{n_{1}, n_{2}}(w,\tau)\bigg\}.\\
\end{align*} 
Выполним замену $F_{n_{1}, n_{2}}(w,\tau)=R_{n_{1}, n_{2}}e^{jwx(\tau)}$, тогда
\begin{equation*}
	\begin{aligned}
		x'(\tau) =
		&\lambda \sum_{n_1=0}^N\sum_{n_2=N-n_1}^{N-n_1} 
		R_{n_{1}, n_{2}}
		- x(\tau)\sum_{n_1=0}^{N-1}\sum_{n_2=0}^{N-1-n_1} 
		R_{n_{1}, n_{2}}+\\
		&+\mu_1 r_2 \sum_{n_1=0}^{N}\sum_{n_2=0}^{N-n_1} 
		n_1 R_{n_{1}, n_{2}}
		+\mu_2 r_2 \sum_{n_1=0}^{N}\sum_{n_2=0}^{N-n_1} 
		n_2 R_{n_{1}, n_{2}}.\\
	\end{aligned}
\end{equation*}
Обозначим через
\begin{equation}\label{a_func}
	\begin{aligned}
		x'(\tau)=a(x)=&\lambda \sum_{n_1=0}^N\sum_{n_2=N-n_1}^{N-n_1} 
		R_{n_{1}, n_{2}}
		- x\sum_{n_1=0}^{N-1}\sum_{n_2=0}^{N-1-n_1} 
		R_{n_{1}, n_{2}}+\\
		&+\mu_1 r_2 \sum_{n_1=0}^{N}\sum_{n_2=0}^{N-n_1} 
		n_1 R_{n_{1}, n_{2}}
		+\mu_2 r_2 \sum_{n_1=0}^{N}\sum_{n_2=0}^{N-n_1} 
		n_2 R_{n_{1}, n_{2}}.
	\end{aligned}
\end{equation}

Теорема доказана.