\begin{equation}\label{hFirstEquation0}
\diffp{H_{0,0}(u,t)}{t}=
	-\lambda H_{0, 0}(u,t) + j\sigma\diffp{H_{0,0}(u,t)}{u}
	+ \mu_1 r_0 H_{1,0}+\mu_2 r_0 H_{0,1}
	+ \mu_1 r_2 e^{ju} H_{1,0} + \mu_2 r_2 e^{ju} H_{0,1}
\end{equation}

\begin{equation}\label{hFirstEquation1}
\begin{aligned}
&\forall n_2 \in [1;N-1]:\\
\diffp{H_{0, n_2}(u,t)}{t}=
	&-(\lambda+n_2\mu_2)H_{0, n_2}(u,t) + j\sigma\diffp{H_{0, n_2}(u,t)}{u}
		+n_2 \mu_2 r_1 (1-q) H_{0, n_2}(u,t)+\\ 
	&+ \lambda (1-q)H_{0, n_2-1}(u,t) 
		- j \sigma (1-q) e^{-ju} \diffp{H_{0, n_2-1}(u,t)}{u} +\\
	&+\mu_1 r_0 H_{1 , n_2}(u,t) 
		+ \mu_{1} r_{2} e^{ju}H_{1, n_2}(u,t)+\\
	&+(n_2+1) \mu_2 r_0 H_{0, n_2 + 1}(u,t) 
		+ (n_2+1) \mu_2 r_2 e^{ju} H_{0, n_2 + 1}(u,t)+\\
	&+\mu_1 r_1(1-q) H_{1 , n_2-1}(u,t)
\end{aligned}
\end{equation}

\begin{equation}\label{hFirstEquation2}
\begin{aligned}
&\forall n_1 \in [1;N-1]:\\
\diffp{H_{n_1, 0}(u,t)}{t}=
	&-(\lambda+n_1\mu_1)H_{n_1, 0}(u,t) + j\sigma \diffp{H_{n_1, 0}(u,t)}{u}
		+n_1 \mu_1 r_1 q H_{n_1, 0}(u,t)+\\ 
	&+ \lambda q H_{n_1-1, 0}(u,t) 
		- j \sigma q e^{-ju} \diffp{H_{n_1-1, 0}(u,t)}{u} +\\
	&+(n_1 + 1)\mu_1 r_0 H_{n_1+1, 0}(u,t) 
		+(n_1 + 1) \mu_{1} r_{2} e^{ju}H_{n_1+1, 0}(u,t)+\\
	&+\mu_2 r_0 H_{n_1, 1}(u,t) 
		+\mu_2 r_2 e^{ju} H_{n_1, 1}(u,t)+\\
	&+\mu_1 r_1 q H_{n_1-1 , 1}(u,t)
\end{aligned}
\end{equation}

\begin{equation}\label{hFirstEquation3}
\begin{aligned}
&\forall n_1, n_2 \in [1;N-1], \text{для которых } n_1+n_2<N:\\
\diffp{H_{n_1, n_2}(u,t)}{t}=
	&-(\lambda+n_1\mu_1+n_2\mu_2)H_{n_1, n_2}(u,t) 
		+ j\sigma\diffp{H_{n_1, n_2}(u,t)}{u}+\\
	&+ n_1 \mu_1 r_1 q H_{n_1, n_2}(u,t)+ n_2\mu_2 r_1 (1-q) H_{n_1, n_2}(u,t)+
		\lambda e^{ju} H_{n_1, n_2}(u,t)+\\
	&+\lambda qH_{n_1-1, n_2}(u,t) 
		- j \sigma q  e^{-ju} \diffp{H_{n_1-1, n_2}(u,t)}{u}+\\
	&+\lambda (1-q)H_{n_1, n_2-1}(u,t) 
		- j \sigma (1-q) e^{-ju} \diff{H_{n_1, n_2-1}(u,t)}{u}+\\
	&+(n_1+1) \mu_1 r_0 H_{n_1 +1 , n_2}(u,t) 
		+ \mu_1 r_2 (n_1+1) e^{ju}H_{n_1 + 1, n_2}(u,t)+\\
	&+(n_2+1) \mu_2 r_0 H_{n_1, n_2 + 1 }(u,t) 
		+ \mu_2 r_2 (n_2+1) e^{ju} H_{n_1, n_2 + 1}(u,t)+\\
	&+(n_1+1)\mu_1 r_1 (1-p) H_{n_1 +1 , n_2-1}(u,t)
		+ (n_2+1)\mu_2 r_{1}q H_{n_1 -1 , n_2+1}(u,t)
\end{aligned}
\end{equation}

\begin{equation}\label{hFirstEquation4}
\begin{aligned}
\diffp{H_{0, N}(u,t)}{t}=
	&-(\lambda+N\mu_2)H_{0, N}(u,t)+N \mu_2 r_1 q H_{0, N}(u,t) 
		+\lambda e^{ju} H_{0, N}(u,t)+\\ 
	&+ \lambda (1-q) H_{0, N-1}(u,t) 
		- j \sigma (1-q) e^{-ju} \diffp{H_{0, N-1}(u,t)}{u} +\\
	&+\mu_2 r_1 (1-q) H_{1 , N-1}(u,t)
\end{aligned}
\end{equation}

\begin{equation}\label{hFirstEquation5}
\begin{aligned}
\diffp{H_{N, 0}(u,t)}{t}=
	&-(\lambda+N\mu_1)H_{N, 0}(u,t)+N \mu_1 r_1 q H_{N, 0}(u,t) 
		+\lambda e^{ju} H_{N, 0}(u,t)+\\ 
	&+ \lambda q H_{N-1, 0}(u,t) 
		- j \sigma q e^{-ju} \diffp{H_{N-1, 0}(u,t)}{u} +\\
	&+\mu_1 r_1 q H_{N-1 , 1}(u,t)
\end{aligned}
\end{equation}

\begin{equation}\label{hFirstEquation6}
\begin{aligned}
&\forall n_1 \in [1;N-1]\\
\diffp{H_{n_1, N-n_1}(u,t)}{t}=
&-(\lambda+n_1\mu_1+(N-n_1)\mu_2)H_{n_1, N-n_1}(u,t) 
		+ j\sigma\diffp{H_{n_1, N-n_1}(u,t)}{u}+\\
	&+ n_1 \mu_1 r_1 q H_{n_1, N-n_1}(u,t)
		+ (N-n_1)\mu_2 r_1 (1-q) H_{n_1, N-n_1}(u,t)+\\
	&+\lambda e^{ju} H_{n_1, N-n_1}(u,t)
		+\lambda qH_{n_1-1, N-n_1}(u,t) 
		- j \sigma q  e^{-ju} \diffp{H_{n_1-1, N-n_1}(u,t)}{u}+\\
	&+\lambda (1-q)H_{n_1, N-n_1-1}(u,t) 
		- j \sigma (1-q) e^{-ju} \diff{H_{n_1, N-n_1-1}(u,t)}{u}+\\
	&+(n_1+1)\mu_1 r_1 (1-p) H_{n_1 + 1 , N - n_1 -1}(u,t)
		+ (N - n_1 +1)\mu_2 r_{1}q H_{n_1 - 1 , N - n_1 +1}(u,t)
\end{aligned}
\end{equation}

