\textbf{Доказательство.}
Подставим $b(x)$ в \eqref{predB}
\begin{equation}\label{withB}
	\begin{split}
		& \frac{\partial \Phi (w,\tau) /\partial\tau}{ \Phi (w,\tau)}=
		\frac{(j w)^2}{2}\Phi (w,\tau)b(x)-w \frac{\partial \Phi (w,\tau)/\partial w}{ \Phi (w,\tau)}\bigg[\lambda\sum_{n_1=0}^N\sum_{n_2=0}^{N-n_1}\varphi_{n_{1}, n_{2}}+\\
		&+\mu_{1}r_{2}\sum_{n_1=0}^{N}\sum_{n_2=0}^{N-n_1}n_{1}\varphi_{n_{1}, n_{2}}+\mu_{2}r_{2}\sum_{n_1=0}^{N}\sum_{n_2=0}^{N-n_1}n_{2}\varphi_{n_{1}, n_{2}}-\\
		&-x\sum_{n_1=0}^{N-1}\sum_{n_2=0}^{N-n_1-1}\varphi_{n_{1}, n_{2}}-\sum_{n_1=0}^{N-1}\sum_{n_2=0}^{N-n_1-1}R_{n_{1}, n_{2}}\bigg].
	\end{split}
\end{equation}
Рассмотрим
\begin{equation*}
	\begin{split}
		&\lambda\sum_{n_1=0}^N\sum_{n_2=0}^{N-n_1}\varphi_{n_{1}, n_{2}}+\mu_{1}r_{2}\sum_{n_1=0}^{N}\sum_{n_2=0}^{N-n_1}n_{1}\varphi_{n_{1}, n_{2}}+\\
		&+\mu_{2}r_{2}\sum_{n_1=0}^{N}\sum_{n_2=0}^{N-n_1}n_{2}\varphi_{n_{1}, n_{2}}-x\sum_{n_1=0}^{N-1}\sum_{n_2=0}^{N-n_1-1}\varphi_{n_{1}, n_{2}}-\sum_{n_1=0}^{N-1}\sum_{n_2=0}^{N-n_1-1}R_{n_{1}, n_{2}}.
	\end{split}
\end{equation*}

Подставим \eqref{solutionPhi} в последнее выражение, получим

\begin{equation}\label{parthWithA}
	\begin{split}
		&\lambda\sum_{n_1=0}^N\sum_{n_2=0}^{N-n_1}\diffp{R_{n_{1}, n_{2}}}{x}+\mu_{1}r_{2}\sum_{n_1=0}^{N}\sum_{n_2=0}^{N-n_1}n_{1}\diffp{R_{n_{1}, n_{2}}}{x}+\mu_{2}r_{2}\sum_{n_1=0}^{N}\sum_{n_2=0}^{N-n_1}n_{2}\diffp{R_{n_{1}, n_{2}}}{x}-\\
		&-x\sum_{n_1=0}^{N-1}\sum_{n_2=0}^{N-n_1-1}\diffp{R_{n_{1}, n_{2}}}{x}-\sum_{n_1=0}^{N-1}\sum_{n_2=0}^{N-n_1-1}R_{n_{1}, n_{2}}.
	\end{split}
\end{equation}

Рассмотрим функцию $a(x)$, найдем ее производную по $x$, учитывая, что $R_{n_1, n_2}$, как решение зависит от $x$

\begin{equation*}
	\begin{aligned}\
		a'(x)=&\lambda \sum_{n_1=0}^N\sum_{n_2=N-n_1}^{N-n_1} 
		\diffp{R_{n_{1}, n_{2}}}{x}
		- x\sum_{n_1=0}^{N-1}\sum_{n_2=0}^{N-1-n_1} 
		\diffp{R_{n_{1}, n_{2}}}{x}- \sum_{n_1=0}^{N-1}\sum_{n_2=0}^{N-1-n_1}R_{n_{1}, n_{2}}+\\
		&+\mu_1 r_2 \sum_{n_1=0}^{N}\sum_{n_2=0}^{N-n_1} 
		n_1 \diffp{R_{n_{1}, n_{2}}}{x}
		+\mu_2 r_2 \sum_{n_1=0}^{N}\sum_{n_2=0}^{N-n_1} 
		n_2 \diffp{R_{n_{1}, n_{2}}}{x}.
	\end{aligned}
\end{equation*}